---
title: 0-Y从0到我不会，长大后再学习
description: 序数
author: VeryrrDefine
date: 2025-4-20 19:04:00 +0800
categories: [Googology]
tags: [googology]
pin: true
math: true
mermaid: true
---
# 0-Y 分析

$$
\begin{array}{l}
() = 0\\
(1) = 1\\
(1,1) = 2\\
(1,2) = \omega\\
(1,2,1) = \omega+1\\
(1,2,1,2) = \omega2\\
(1,2,1,2,1,2) = \omega3\\
(1,2,1,2,1,2,\cdots) = (1,2,2) = \omega^2\\
(1,2,2,1,2) = \omega^2+\omega\\
(1,2,2,1,2,2) = \omega^2 2\\
(1,2,2,2) = \omega^3\\
(1,2,2,2,2) = \omega^4\\
(1,2,3) = (1,2,2,\cdots) = \omega^\omega\\
(1,2,3,2) = \omega^{\omega+1}\\
(1,2,3,2,2) = \omega^{\omega+2}\\
(1,2,3,2,3) = (1,2,3,2,2,\cdots) = \omega^{\omega 2}\\
(1,2,3,2,3,2) = \omega^{\omega 2+1}\\
(1,2,3,2,3,2,3) = \omega^{\omega 3}\\
(1,2,3,3) = \omega^{\omega^2}\\
(1,2,3,3,2,3) = \omega^{\omega^2+\omega}\\
(1,2,3,3,2,3,3) = \omega^{\omega^2 2}\\
(1,2,3,3,3) = \omega^{\omega^3}\\
(1,2,3,4) = \omega^{\omega^\omega}\\
(1,2,3,4,4) = \omega^{\omega^{\omega^2}}\\
(1,2,3,4,5) = \omega^{\omega^{\omega^\omega}}\\

(1,3) = (1,2,3,4,\cdots) = \varepsilon_{0} = \psi(\Omega)\\
(1,3,2) = (1,3,1,3,\cdots) = \varepsilon_0 \omega = \psi(\Omega+1)\\
(1,3,2,2) = \varepsilon_0 \omega^2 = \psi(\Omega+2)\\
(1,3,2,3) = \varepsilon_0 \omega^\omega = \psi(\Omega+\omega)\\
(1,3,2,3,4) = \varepsilon_0 \omega^{\omega^\omega} = \psi(\Omega+\omega^\omega)\\
(1,3,2,4) = \varepsilon_0^2 = \psi(\Omega+\psi(\Omega)\\
(1,3,2,4,2) = \varepsilon_0^2\omega = \psi(\Omega+\psi(\Omega)+1)\\
(1,3,2,4,2,3) = \varepsilon_0^2\omega^\omega = \psi(\Omega+\psi(\Omega)+\omega)\\
(1,3,2,4,2,4) = \varepsilon_0^3 = \psi(\Omega+\psi(\Omega)2)\\
(1,3,2,4,3) = \varepsilon_0^\omega = \psi(\Omega+\psi(\Omega+1))\\


\end{array}

$$
